
\section{Instances of Functor, Applicative, Monad}

Show that monadic streams are an instance of these three classes, under some assumptions about the underlying monad.

So far we determined that we think that MonStr satisfies the monad laws if the underlying monad is commutative and idempotent \cite{idempotent_monads}. (Proof?)

What about Applicative?

Give conterexamples where it isn't a monad (using State).

Also examples when it is a monad even if the underlying monad is not commutative and idempotent: with List as underlying monad we obtain Trees, which are a monad. Can this be generalized.

This section outlines the Functor, Applicative, and Comonad instances

\subsection{Functor Instance}

To show that $\stream{M}$ is a functor whenever $M$ is, we have to define its behaviour on morphisms: if $f:A\rightarrow B$, then we must define how $f$ maps on monadic streams:
$$
\begin{array}{l}
\stream{M}\,f : \stream{M,A} \rightarrow \stream{M,B}\\
\stream{M}\,f\,(\mcons\,m) = \mcons\,(M\,(f\times \stream{M}\,f)\,m)
\end{array}
$$

This definition doesn't strictly comply with the {\em guarded-by-constructors} discipline: the recursive call to $(\stream{M}\,f)$ doesn't occur directly as an argument to the constructor $\mcons$, but it is below the $\times$ operator and an application of $M$.
However, this is just the application of the functor $M\,(- \times -)$ which defines the final coalgebras. In other words, this is actually how we determine the positions in the container tree.
\begin{vcomment}
	This is very badly explained: needs more extensive clarification.
\end{vcomment}
















\subsection{Functor instance in Haskell}

\begin{haskell}
unwrapMS :: MonStr m a -> m (a, MonStr m a)
unwrapMS (MCons m) = m

transformMS :: Functor m => (a -> MonStr m a -> (b, MonStr m b)) ->
                                  MonStr m a -> MonStr m b
transformMS f s = MCons $ fmap (\(h,t) -> f h t) (unwrapMS s)

instance Functor m => Functor (MonStr m) where
   -- fmap :: (a -> b) -> MonStr m a -> MonStr m b
   fmap f = transformMS (\a s -> (f a, fmap f s))
\end{haskell}

\subsubsection{Functor proof}

Proof that \hcode{fmap id == id}

\begin{haskell}
fmap id = transformMS (\a s -> id a, fmap id s)
-- definition of `transformMS`
= \s -> MCons $ fmap (\(h,t) -> (\a s -> (id a, fmap id s)) h t) (unwrapMS s)
-- application of `(\a s -> (id a, fmap id s))` to `h t`
= \s -> MCons $ fmap (\(h,t) -> (id h, fmap id t)) (unwrapMS s)
-- take as assumption that `fmap id t == id t` - coinductive hypothesis?
= \s -> MCons $ fmap (\(h,t) -> (id h, id t)) (unwrapMS s)
-- definition of `id`
= \s -> MCons $ fmap (\(h,t) -> (h,t)) (unwrapMS s)
-- definition of `id`
= \s -> MCons $ fmap id (unwrapMS s)
-- `unwrapMS` returns an element in a functor, so `fmap id == id` in this case
= \s -> MCons $ id (unwrapMS s)
-- application of `id`
= \s -> MCons $ (unwrapMS s)
-- MCons and unwrapMS are inverses
= \s -> id s 
= id
\end{haskell}

Proof that \verb+fmap (f . g) == (fmap f) . (fmap g)+

To simplify notation in the proof, we introduce the notation \verb+tr(f)+ for the expression \verb+\(h,t) -> (f h, fmap f t)+.

We're going to use the fact that the underlying operator \verb+m+ is a functor and so satisfies the functor laws, and also that the pairing operator \verb+(,)+ is functorial in both arguments.

By definition of \verb+fmap+ for monsters, we have that
\begin{haskell}
fmap f s = transformMS (\ a s -> (f a, fmap f s)) s
         = MCons $ fmap (\ (h,t) -> (\a s -> (f a, fmap f s) h t)) (unwrapMS s)
         = MCons $ fmap (\ (h,t) -> (f h, fmap f t)) (unwrapMS s)
         = MCons $ fmap tr(f) (unwrapMS s)
\end{haskell}

We also use the fact that the monster constructor \verb+MCons+ and the function \verb+unwrapMS+ that removes it are inverse of each other.

\begin{haskell}
fmap (f . g) = transformMS (\a s -> (f . g) a, fmap (f . g) s)
-- definition of `transformMS`
= \s -> MCons $ fmap (\(h,t) -> (\a s -> ((f . g) a, fmap (f . g) s)) h t) (unwrapMS s)
-- application of `(\a s -> ((f . g) a, fmap (f . g) s))` to `h t`
= \s -> MCons $ fmap (\(h,t) -> ((f . g) h, fmap (f . g) t)) (unwrapMS s)`
-- take as assumption that `fmap (f . g) t == (fmap f . fmap g) t` - coinductive hypothesis?
= \s -> MCons $ fmap (\(h,t) -> ((f . g) h, (fmap f . fmap g) t)) (unwrapMS s)
-- By fuctoriality of pairing in both components
= \s -> MCons $ fmap (tr(f) . tr(g)) (unwrapMS s)
-- By functoriality of the underlying operator m
= \s -> MCons $ (fmap tr(f)) . (fmap tr(g)) (unwrapMS s)
-- MCons and unwrapMS are inverses
= \s -> MCons $ fmap tr(f)) $ unwrapMS $ MCons $ fmap tr(g) (unwrapMS s)
= \s -> MCons $ fmap tr(f)) $ unwrapMS $ fmap g s
= \s -> fmap f $ fmap g s
= fmap f . fmap g
\end{haskell}

\subsection{Applicative instance in Haskell}

\begin{haskell}
unwrapMS :: MonStr m a -> m (a, MonStr m a)
unwrapMS (MCons m) = m

transformMS :: Functor m => (a -> MonStr m a -> (b, MonStr m b)) ->
                                  MonStr m a -> MonStr m b
transformMS f s = MCons $ fmap (\(h,t) -> f h t) (unwrapMS s)

instance Functor m => Functor (MonStr m) where
   -- fmap :: (a -> b) -> MonStr m a -> MonStr m b
   fmap f = transformMS (\a s -> (f a, fmap f s))
\end{haskell}

\subsection{Comonad instance in Haskell}

\begin{haskell}
instance Comonad w => Comonad (MonStr w) where
  --extract :: MonStr w a -> a
  extract = extract . headMS
  
  --duplicate :: MonStr w a -> MonStr w (MonStr w a)
  duplicate s = MCons $ fmap (\(h,t) -> (s, duplicate t)) (unwrapMS s)
\end{haskell}

\verb+headMS+ returns the first element of the first pair in the monster, wrapped in the underlying functor. Since this functor is required to be a comonad, extract can be used to return the wrapped values inside.

We introduce \verb+mm(s)+ for the "monster matrix" formed by a monadic stream \verb+s+ - this is defined as a monster where the first element is \verb+s+, the second is the tail of \verb+s+, the third is the tail of the tail of \verb+s+, and so on.

The \verb+duplicate+ instance for monadic streams forms this "monster matrix": \verb+duplicate s = mm(s)+

\subsubsection{Comonad law proofs}

Proof that \verb+extract . duplicate == id+

\begin{haskell}
extract . duplicate 
= \ms -> extract (MCons $ fmap (\(h,t) -> (ms, duplicate t)) 
	(unwrapMS ms))
= \ms -> extract (headMS (MCons $ fmap (\(h,t) -> (ms, duplicate t)) 
	(unwrapMS ms)))
= \ms -> ms 
= id
\end{haskell}

Proof that \verb+fmap extract . duplicate == id+

\begin{haskell}
fmap extract . duplicate = \ms -> fmap extract (MCons $ fmap (\(h,t) -> 
	(ms, duplicate t)) (unwrapMS ms))
= \ms -> transformMS (\a s -> (extract a, fmap extract s)) (MCons $ 
	fmap (\(h,t) -> (ms, duplicate t)) (unwrapMS ms))
  [transformMS definition]
= \ms -> MCons $ fmap (\(h,t) -> (extract h, fmap extract t)) 
	(fmap (\(h,t) -> (ms, duplicate t)) (unwrapMS ms)) 
= \ms -> MCons $ fmap (\(h,t) -> (extract ms, fmap extract (duplicate t))) 
	(unwrapMS ms)
  [coinductive hypothesis]
= \ms -> MCons $ fmap (\(h,t) -> ((extract . headMS) ms, id t)) (unwrapMS ms)
  [(extract . headMS) ms = a, first element of ms]
= \ms -> MCons $ fmap (\(h,t) -> (a, id t)) (unwrapMS ms)
  [a is defined as the first element of ms, so h = a under the fmap]
= \ms -> ms
= id
\end{haskell}

Proof that \verb+duplicate . duplicate == fmap duplicate . duplicate+

\begin{haskell}
duplicate . duplicate = \ms -> duplicate (duplicate ms)
= \ms -> MCons $ fmap (\(h,t) -> (duplicate ms, duplicate t)) $
	(fmap (\(h,t) -> (ms, duplicate t)) (unwrapMS ms))
= \ms -> MCons $ fmap ((\(h,t) -> (duplicate ms, duplicate (duplicate t))) 
	(unwrapMS ms)
                      
fmap duplicate . duplicate = \ms -> fmap duplicate (MCons $ fmap (\(h,t) -> 
	(ms, duplicate t)) (unwrapMS ms))
= \ms -> transformMS (\a s -> (duplicate a, fmap duplicate s)) $
	(MCons $ fmap (\(h,t) -> (ms, duplicate t)) (unwrapMS ms))
= \ms -> MCons $ fmap (\(h,t) -> (\a s -> 
	(duplicate a, fmap duplicate s)) h t) (unwrapMS (MCons $ fmap (\(h,t) -> 
	(ms, duplicate t)) (unwrapMS ms)))
= \ms -> MCons $ fmap (\(h,t) -> (duplicate h, fmap duplicate t)) $ 
	(fmap (\(h,t) -> (ms, duplicate t)) (unwrapMS ms))
= \ms -> MCons $ fmap (\(h,t) -> 
	(duplicate ms, fmap duplicate (duplicate t))) (unwrapMS ms)
  [coinductive hypothesis]
= \ms -> MCons $ fmap ((\(h,t) -> 
	(duplicate ms, duplicate (duplicate t))) (unwrapMS ms)
= duplicate . duplicate
\end{haskell}


%\section{Monad proof}
%\input{monster_article_monad_proof}
